generational/spec/GC.Gen.HeapExtensional.fsti
@@ -1,0 +1,14 @@
+module GC.Gen.HeapExtensional
+
+open FStar.Seq
+module U64 = FStar.UInt64
+
+open GC.Spec.Base
+open GC.Spec.Heap
+
+val heap_read_word_ext (h1 h2: heap)
+  : Lemma
+    (requires (forall (a: nat).
+       a < heap_size /\ a % 8 == 0 ==>
+       read_word h1 (U64.uint_to_t a) == read_word h2 (U64.uint_to_t a)))
+    (ensures h1 == h2)
